---
title: Test
description: Test description
date: 2024-10-24 11:33:00 +0800
categories:
  - Blogging
  - Demo
tags:
  - typography
pin: true
math: true
mermaid: true
---

#### Problem 1.1: Show that $(\text{G}, *)$ is an abelian group
###### Part a 
> Let $\text{G}=\mathbb{Q} \setminus \{ -6 \}$

> $\forall x,y \in G: x*y=90xy+540x+540y+3234$

- **First we show that $*$ is a binary operation.**
$$
\begin{align}
x*y&=90xy+540x+540y+3234 \\
&=90x(y+6)+540(y+6) - 6 \\
&=90(x+6)(y+6) - 6 \\
\end{align}
$$

Because $x \neq-6$ and $y \neq -6$, we have $90(x+6)(y+6) -6 \neq -6$, so $x * y  \in\mathbb{Q}\setminus \left\lbrace -6 \right\rbrace$.
Which proves that $*$ is a binary operation.

- **Next we show that $*$ is associative.**

Suppose $x, y, z \in \text{G}$, we have
$$
\begin{align}
(x * y) * z &= (90(x+6)(y+6)-6) * z  \\
&= 90(90(x+6)(y+6))(z+6)-6 \\
&= 90(x+6)(90(y+6)(z+6))-6 \\
&= x * (90(y+6)(z+6)-6) \\
&= x * (y * z) \\
\end{align}
$$
This proves that $*$ is associative.

- **Next we show that $*$ is commutative.**

Suppose $x, y\in \text{G}$, we have
$$
\begin{align}
x * y &= 90(x+6)(y+6)-6 \\
 &= 90(y+6)(x+6)-6 \\
 &= y * x\\
\end{align}
$$
This proves that $*$ is commutative.

- **Next we show that there exists an element $e \in \text{G}$ such that $a * e=e * a=a$.**
$$
\begin{align}
a*e&=a \\
90(a+6)(e+6)-6&=a \\
e+6&=\frac{a+6}{90(a+6)} \\
e&=\frac{1}{90}-6=-\frac{539}{90} \\
\end{align}
$$

So with $e =-\displaystyle\frac{539}{60} \in \text{G}$, $a * e=a$, and because $*$ is commutative, so $a * e=e * a=a$.
So this proves that there is an identity element $e=-\displaystyle\frac{539}{90}$.

- **Next, we show that every element $x \in \text{G}$, there exists an element $x^{-1} \in \text{G}$ such that $x * x^{-1} =e$.**
$$
\begin{align}
x * x^{-1} &= e \\
90(x+6)(x^{-1} +6)-6 &= -\frac{539}{90} \\
90(x+6)(x^{-1} +6) &= \frac{1}{90} \\
x^{-1} &= \frac{1}{8100(x+6)} - 6 \\
\end{align}
$$

Since $\displaystyle\frac{1}{8100(x+6)} \neq 0$, so $x^{-1} \neq -6$, so $x^{-1} \in \text{G}$.
This proves that there exists an inverse for all elements in the group.

So we can see that $\text{G}$ is indeed an abelian group.

###### Part b
> Let $\text{G}=(0,+\infty)\setminus \{ 1 \}$

> $\forall x,y \in \text{G}\colon x*y=x^{\log y}$

- **First, we show that $*$ is a binary operation on $\text{G}$.**

We need to show that for all $x, y \in \text{G}$, $x*y \in \text{G}$.

Given that $x > 0$, $x \neq 1$, and $y > 0$, $y \neq 1$.

Compute:
$$
x * y = x^{\log y}
$$

Since $x > 0$ and $\log y$ is defined for $y > 0$, $x^{\log y} > 0$.

Suppose $x^{\log y} = 1$. Then:
$$
\begin{align}
\log(x^{\log y}) &= \log 1 \\
(\log y)(\log x) &= 0
\end{align}
$$
Since $x \neq 1$, we have $\log x \neq 0$, the same with $y$, we have $\log y \neq 0$, yet their product is $0$, which contradicts the assumption that $x^{\log y} = 1$.

Therefore, $x^{\log y} \neq 1$, and thus $x*y \in \text{G}$.

- **Next, we show that $*$ is associative.**

For all $x, y, z \in \text{G}$, we have:
$$
\begin{align}
(x * y) * z &= (x^{\log y})^{\log z} = x^{\log y \cdot \log z} \\
&= x^{\log z \cdot\log y} = x^{\log(y^{\log z})} \\
&= x^{\log \left( y *z \right) } = x * (y * z)
\end{align}
$$
This shows that $*$ is associative.

- **Next, we show that $*$ is commutative.**

For all $x, y \in \text{G}$, we have:
$$
\begin{align}
x * y &= x^{\log y} = e^{\log x \cdot \log y} \\
&= e^{\log y \cdot \log x} = y^{\log x} \\
&= y * x
\end{align}
$$
This shows that $*$ is commutative.

- **Next, we show that there exists an identity element $u \in \text{G}$ such that $x * u = x$.**

We need to find $u \in \text{G}$ such that:
$$
\begin{align}
x * u &= x \\
x^{\log u} &= x \\
\log(x^{\log u}) &= \log x \\
(\log u)(\log x) &= \log x \\
\log u &= 1 \\
u &= e \\
\end{align}
$$
Thus, the identity element is $u = e$.

Since $e \in (0, +\infty) \setminus \{1\}$, we have $u \in \text{G}$.

- **Next, we show that for each $x \in \text{G}$, there exists an inverse $x^{-1} \in \text{G}$ such that $x * x^{-1} = u$.**

$$
\begin{align}
x * x^{-1} &= u \\
x^{\log x^{-1}} &= u \\
x^{\log x^{-1}} &= e \\
\log(x^{\log x^{-1}}) &= 1 \\
(\log x)(\log x^{-1}) &= 1\\
\log x^{-1} &= \frac{1}{\log x}\\
x^{-1} &= e^{\frac{1}{\log x}}
\end{align}
$$

Since $x \in \text{G}$, $\log x \neq 0$, so $x^{-1} \in (0,+\infty)$.

Also, $x^{-1} \neq 1$ because if $x^{-1} = 1$, then $\log x^{-1} = 0$, which contradicts $\log x^{-1} = \frac{1}{\log x} \neq 0$.

Therefore, $x^{-1} \in \text{G}$.

This shows that inverses exist for all elements in $\text{G}$.

###### Part c
> Let $\text{G}=\mathbb{R}\text{ and } n \text{ is odd}$

> $\forall x, y \in \text{G}\colon x*y=\sqrt[n]{ x^{n} +y^{n}}$

- **First, we show that $*$ is a binary operation on $\text{G}$.**

Since $n$ is odd, the $n$-th root $\sqrt[n]{\cdot}$ is defined for all real numbers. For all $x, y \in \mathbb{R}$:
$$
x * y = \sqrt[n]{x^{n} + y^{n}} \in \mathbb{R}
$$

- **Next, we show that $*$ is associative.**

For all $x, y, z \in \text{G}$:
$$
\begin{align}
(x * y) * z &= \sqrt[n]{(x * y)^{n} + z^{n}} = \sqrt[n]{(x^{n} + y^{n}) + z^{n}} \\
&= \sqrt[n]{x^{n} + y^{n} + z^{n}} = x * (y * z)
\end{align}
$$

- **Next, we show that $*$ is commutative.**

For all $x, y \in \text{G}$:
$$
x * y = \sqrt[n]{x^{n} + y^{n}} = \sqrt[n]{y^{n} + x^{n}} = y * x
$$

- **Next, we show that there exists an identity element $e \in \text{G}$ such that $x * e = x$.**

We need to find $e \in \text{G}$ such that:
$$
\begin{align}
x * e &= x  \\
\sqrt[n]{x^{n} + e^{n}} &= x\\
 x^{n} + e^{n} &= x^{n}  \\
 e^{n} &= 0  \\
 e &= 0
\end{align}
$$
Therefore, the identity element is $e = 0$, and $x*e=e*x=x$.

- **Next, we show that every element $x \in \text{G}$ has an inverse $x^{-1} \in \text{G}$ such that $x * x^{-1} = e$.**

We need to find $x^{-1} \in \text{G}$ such that:
$$
\begin{align}
\sqrt[n]{x^{n} + (x^{-1})^{n}} &= 0 \\
 x^{n} + (x^{-1})^{n} &= 0  \\
 (x^{-1})^{n} &= -x^{n} \\
x^{-1} &= -x \hspace{24pt} \text{ (Since $n$ is odd) }
\end{align}
$$
Thus, the inverse of $x$ is $x^{-1} = -x$.

Therefore, $(\text{G}, *)$ is an abelian group.

###### Part d
> Let $\text{G}$ be $\mathbb{R}$ and $n$ be an odd number.

> $\forall x,y \in \text{G}\colon x*y=(\sqrt[n]{ x }+\sqrt[n]{ y })^{n}$

- **First, we show that $*$ is a binary operation on $\text{G}$.**

Since $n$ is odd, $\sqrt[n]{x}$ is defined for all $x \in \mathbb{R}$. Therefore:
$$
x * y = \left( \sqrt[n]{x} + \sqrt[n]{y} \right)^{n} \in \mathbb{R}
$$

- **Next, we show that $*$ is associative.**

For all $x, y, z \in \text{G}$:
$$
\begin{align}
(x * y) * z &= \left( \sqrt[n]{x * y} + \sqrt[n]{z} \right)^{n} \\
&= \left( \sqrt[n]{ \left( \sqrt[n]{x} + \sqrt[n]{y} \right)^{n} } + \sqrt[n]{z} \right)^{n} \\
&= \left( \sqrt[n]{x} + \sqrt[n]{y} + \sqrt[n]{z} \right)^{n} = x * (y * z)
\end{align}
$$

- **Next, we show that $*$ is commutative.**

For all $x, y \in \text{G}$:
$$
x * y = \left( \sqrt[n]{x} + \sqrt[n]{y} \right)^{n} = \left( \sqrt[n]{y} + \sqrt[n]{x} \right)^{n} = y * x
$$

- **Next, we show that there exists an identity element $e \in \text{G}$ such that $x * e = x$.**

We need to find $e \in \text{G}$ such that:
$$
\begin{align}
\left( \sqrt[n]{x} + \sqrt[n]{e} \right)^{n} &= x  \\
 \sqrt[n]{x} + \sqrt[n]{e} &= \sqrt[n]{x}  \\
 \sqrt[n]{e} &= 0  \\
 e &= 0
\end{align}
$$
Therefore, the identity element is $e = 0$.

- **Next, we show that every element $x \in \text{G}$ has an inverse $x^{-1} \in \text{G}$ such that $x * x^{-1} = e$.**

We need to find $x^{-1} \in \text{G}$ such that:
$$
\begin{align}
\left( \sqrt[n]{x} + \sqrt[n]{x^{-1}} \right)^{n} &= 0 \\
 \sqrt[n]{x^{-1}} &= -\sqrt[n]{x}
\end{align}
$$
Since $n$ is odd:
$$
x^{-1} = \left( -\sqrt[n]{x} \right)^{n} = -x
$$
Thus, the inverse of $x$ is $x^{-1} = -x$.

Therefore, $(\text{G}, *)$ is an abelian group.

#### Problem 1.2

> Let $(\text{G}, * )$ be a group. Assume $a \in \text{G}$. $\forall x,y \in \text{G}$, put $x \cdot y=x * a * y$,

> Show that $(\text{G}, \cdot)$ is a group.

- **First, we show that $\cdot$ is a binary operation on $\text{G}$.**

Since $x, a, y \in \text{G}$ and $\text{G}$ is closed under $*$, we have $x \cdot y = x * a * y \in \text{G}$.

- **Next, we show that $\cdot$ is associative.**

For all $x, y, z \in \text{G}$:
$$
\begin{align}
(x \cdot y) \cdot z &= (x * a * y) \cdot z  \\
&= (x * a * y) * a * z \\
&= x * a * y * a * z \quad (\text{since $*$ is associative}) \\
&= x * a * (y * a * z) \\
&= x \cdot (y \cdot z)
\end{align}
$$

- **Next, we find the identity element $e' \in \text{G}$ such that $x \cdot e' = x$ and $e' \cdot x = x$.**

We need:
$$
\begin{align}
x \cdot e' &= x \\
x * a * e' &= x \\
a * e' &= e  \\
e' &= a^{-1}
\end{align}
$$
Similarly:
$$
\begin{align}
e' \cdot x &= x \\
e' * a * x &= x \\
e' * a &= e  \\
e' &= a^{-1}
\end{align}
$$
Therefore, the identity element is $e' = a^{-1}$.

- **Next, we show that every element $x \in \text{G}$ has an inverse $x^{\prime} \in \text{G}$ such that $x \cdot x^{\prime} = e'$.**

We need to find $x^{\prime} \in \text{G}$ such that:
$$
\begin{align}
x \cdot x^{\prime} &= e' \\
x \cdot x^{\prime} &= a^{-1}  \\
x * a * x^{\prime} &= a^{-1} \\
x^{\prime} &= a^{-1} * x^{-1} * a^{-1}
\end{align}
$$
Since $x^{\prime} \in \text{G}$, inverses exist.

Therefore, $(\text{G}, \cdot)$ is a group.

#### Problem 1.3
> Let $(\text{G}, \cdot)$ be a group. Assume that $\exists n \geq 1$ such that:
$$
\begin{align}
(xy)^{n}&=x^{n}y^{n} \\
(xy)^{n+1}&=x^{n+1}y^{n+1} \\
\text{and} (xy)^{n+2}&=x^{n+2}y^{n+2}
\end{align}
$$
> Show that $\text{G}$ is abelian.

- **Since $\text{G}$ is already a group, we only need to show that $x y = y x$ for all $x, y \in \text{G}$.**

$$
\begin{align}
(xy)^{n+2} &= x^{n+2}y^{n+2} \\
xy(xy)^{n}xy &= x^{n+2}y^{n+2} \\
y(xy)^{n}x &= x^{n+1}y^{n+1} \\
(yx)^{n+1} &= x^{n+1}y^{n+1} \\
(yx)^{n+1} &= (xy)^{n+1} \\
(yx)^{n+1}(yx)^{-n} &= (xy)^{n+1}(xy)^{-n} \\
yx &= xy \hspace{24pt}\text{(Q.E.D)} \\
\end{align}
$$
So $\text{G}$ is abelian.

#### Problem 1.4
> Given

$$
G = \left\{ \begin{pmatrix} x & y \\ 2y & x \end{pmatrix} \colon  x, y \in \mathbb{Q}, x^2 + y^2 > 0 \right\}
$$
> Show that $\text{G}$ is a group with matrix multiplication.

- **First, we show that $\text{G}$ is closed under multiplication.**

Let $$A = \begin{pmatrix} x_1 & y_1 \\ 2 y_1 & x_1 \end{pmatrix}$$ and $$
B = \begin{pmatrix} x_2 & y_2 \\ 2 y_2 & x_2 \end{pmatrix}$$ in $\text{G}$. Compute $A B$:

$$
A B = \begin{pmatrix}
x_1 x_2 + 2 y_1 y_2 & x_1 y_2 + y_1 x_2 \\
2 y_1 x_2 + x_1 2 y_2 & 2 y_1 y_2 + x_1 x_2
\end{pmatrix}
$$

Let $x_3 = x_1 x_2 + 2 y_1 y_2$ and $y_3 = x_1 y_2 + y_1 x_2$. Then:

$$
A B = \begin{pmatrix} x_3 & y_3 \\ 2 y_3 & x_3 \end{pmatrix}
$$

Since $x_3^2 + y_3^2 > 0$, $A B \in \text{G}$.

- **Matrix multiplication is associative**, so associativity holds.

- **Next, we find the identity element $e$ in $\text{G}$.**
The identity matrix is $I = \begin{pmatrix} 1 & 0 \\ 0 & 1 \end{pmatrix}$ under the matrix multiplication operation, which can be written in the form of elements of $\text{G}$ with $x = 1$, $y = 0$. 
So we have $\forall x \in \text{G}\colon ex=xe=x$ with $e= \begin{pmatrix} 1 & 0 \\ 0 & 1 \end{pmatrix}$.

- **Next, we show that every element has an inverse.**
For $A = \begin{pmatrix} x & y \\ 2 y & x \end{pmatrix}$, compute $\det A$:
$$
\det A = x^2 - (2 y)(y) = x^2 - 2 y^2 = (x - \sqrt{ 2 } y)(x + \sqrt{ 2 } y)
$$
The condition $x^2 + y^2 > 0$ already ensures that $x \neq 0$ and $y \neq 0$, so if $\det A = 0$, then the values for $x$ can only be $x = \pm \sqrt{ 2 }y$. But $x, y \in \mathbb{Q}$, so that cannot happen.

From this, we have
$$
\begin{align}
&A^{-1} = \frac{1}{\det A} \begin{pmatrix} x & -y \\ -2 y & x \end{pmatrix} = \begin{pmatrix} x' & y' \\ 2 y' & x' \end{pmatrix} \\[4pt]
&\text{where} \quad x' = \frac{x}{\det A}, \ y' = \frac{-y}{\det A}
\end{align}
$$

So $A^{-1} \in \text{G}$ exists for all $A \in \text{G}$.

Therefore, $\text{G}$ is a group under matrix multiplication.
